lang.v
@@ -13,23 +13,7 @@ Module Lang (C : CORE_LANG).
 
   Export C.
 
-  Delimit Scope lang_scope with lang.
-  Local Open Scope lang_scope.
-
-  (* Notation "'ε'"    := empty_ctx : lang_scope. *)
-  (* Notation "K1 ∘ K2"  := (comp_ctx K1 K2) (at level 40, left associativity) : lang_scope. *)
-
-  (* Arguments fork_not_value {_} _. *)
-  (* Arguments comp_ctx_positive {_ _} _. *)
-  (* Arguments fork_inj {_ _} _. *)
-  (* Arguments fill_inj_r _ {_ _} _. *)
-  (* Arguments fill_value {_ _} _. *)
-  (* Arguments fill_fork {_ _ _} _. *)
-  (* Arguments values_stuck {_} _ {_ _} _ _. *)
-  (* Arguments atomic_reducible {_} _. *)
   Arguments atomic_step {_ _ _ _} _ _ _.
-
-  Local Open Scope lang_scope.
 
   (** Thread pools **)
   Definition tpool : Type := list expr.
@@ -38,109 +22,19 @@ Module Lang (C : CORE_LANG).
   Definition cfg : Type := (tpool * state)%type.
 
   (* Threadpool stepping relation *)
+  Definition option_to_list {A: Type} (o: option A): list A :=
+    match o with
+    | None => []
+    | Some a => [a]
+    end.
+
   Inductive step (ρ ρ' : cfg) : Prop :=
-  | step_atomic : forall e e' σ σ' t1 t2,
+  | step_atomic : forall e e' ef σ σ' t1 t2,
                     ρ  = (t1 ++ e  :: t2, σ) ->
-                    ρ' = (t1 ++ e' :: t2, σ') ->
-                    prim_step (e, σ) (e', σ') None ->
+                    ρ' = (t1 ++ e' :: t2 ++ option_to_list ef, σ') ->
+                    prim_step (e, σ) (e', σ') ef ->
                     step ρ ρ'
-  | step_atomic_fork : forall e e' σ σ' t1 t2 ef,
-                         ρ  = (t1 ++ e :: t2, σ) ->
-                         ρ' = (t1 ++ e' :: t2 ++ ef :: nil, σ') ->
-                         prim_step (e, σ) (e', σ') (Some ef) ->
-      step ρ ρ'
   .
-  
-  (* | step_fork : forall e σ K t1 t2, *)
-  (*     (* thread ID is 0 for the head of the list, new thread gets first free ID *) *)
-  (*     ρ  = (t1 ++ fill K (fork e) :: t2, σ) -> *)
-  (*     ρ' = (t1 ++ fill K fork_ret :: t2 ++ e :: nil, σ) -> *)
-  (*     step ρ ρ'. *)
-
-  (* Lemma comp_ctx_neut_emp_r {K K'} : *)
-  (*   K = K ∘ K' -> *)
-  (*   K' = ε. *)
-  (* Proof. *)
-  (*   intros HEq. *)
-  (*   rewrite <- comp_ctx_emp_r in HEq at 1. *)
-  (*   apply comp_ctx_inj_r in HEq; now symmetry. *)
-  (* Qed. *)
-
-  (* Lemmas about expressions *)
-  Lemma reducible_not_value {e} :
-    reducible e -> ~is_value e.
-  Proof.
-    intros H_red H_val.
-    eapply values_stuck; try eassumption.
-  Qed.
-
-  (* Lemma reducible_not_fork {e K e'} : *)
-  (*   reducible e -> e <> fill K (fork e'). *)
-  (* Proof. *)
-  (*   move=> HRed HDec. *)
-  (*   move: (fork_stuck K e'); rewrite -HDec -(fill_empty e) => HStuck {HDec}. *)
-  (*   exact: (HStuck _ _ eq_refl). *)
-  (* Qed. *)
-
-  (* Lemma step_same_ctx {K K' e e'} : *)
-  (*                        fill K e = fill K' e' -> *)
-  (*                        reducible e  -> *)
-  (*                        reducible e' -> *)
-  (*                        K = K'. *)
-  (* Proof. *)
-  (*   intros H_fill H_red H_red'. *)
-  (*   edestruct (step_by_value K K' e e') as [K'' H_K'']. *)
-  (*   - assumption. *)
-  (*   - assumption. *)
-  (*   - now apply reducible_not_value. *)
-  (*   - edestruct (step_by_value K' K e' e) as [K''' H_K''']. *)
-  (*     + now symmetry. *)
-  (*     + assumption. *)
-  (*     + now apply reducible_not_value. *)
-  (*     + subst K. *)
-  (*       rewrite <- comp_ctx_assoc in H_K''. *)
-  (*       assert (H_emp := comp_ctx_neut_emp_r H_K''). *)
-  (*       apply comp_ctx_positive in H_emp. *)
-  (*       destruct H_emp as[H_K'''_emp H_K''_emp]. *)
-  (*       subst K'' K'''. *)
-  (*       now rewrite comp_ctx_emp_r. *)
-  (* Qed. *)
-
-  Lemma atomic_not_stuck {e} :
-    atomic e -> ~stuck e.
-  Proof.
-    intros H_atomic H_stuck.
-    eapply H_stuck.
-    now eapply atomic_reducible.
-  Qed.
-
-  (* Lemma fork_not_atomic K e : *)
-  (*   ~atomic (fill K (fork e)). *)
-  (* Proof. *)
-  (*   intros HAt. *)
-  (*   apply atomic_not_stuck in HAt. *)
-  (*   apply HAt, fork_stuck. *)
-  (* Qed. *)
-
-  Lemma atomic_not_value e :
-    atomic e -> ~is_value e.
-  Proof.
-    intros HAt HVal.
-    apply atomic_not_stuck in HAt; apply values_stuck in HVal.
-    tauto.
-  Qed.
-
-  (* Lemma atomic_fill {e K} *)
-  (*       (HAt : atomic (fill K e)) *)
-  (*       (HNV : ~ is_value e) : *)
-  (*   K = empty_ctx. *)
-  (* Proof. *)
-  (*   destruct (step_by_value K ε e (fill K e)) as [K' EQK]. *)
-  (*   - now rewrite fill_empty. *)
-  (*   - now apply atomic_reducible. *)
-  (*   - assumption. *)
-  (*   - symmetry in EQK; now apply comp_ctx_positive in EQK. *)
-  (* Qed. *)
 
   (* Reflexive, transitive closure of the step relation *)
   Global Instance cfg_type : Setoid cfg := discreteType.
