core_lang.v
@@ -11,109 +11,35 @@ Module Type CORE_LANG.
   Definition value : Type := {e: expr | is_value e}.
   Parameter is_value_dec : forall e, is_value e + ~is_value e.
 
-  (* fork and fRet *)
-  (* Parameter fork : expr -> expr. *)
-  (* Parameter fork_ret : expr. *)
-  (* Axiom fork_ret_is_value : is_value fork_ret. *)
-  (* Definition fork_ret_val : value := exist _ fork_ret fork_ret_is_value. *)
-  (* Axiom fork_not_value : forall e, *)
-  (*                          ~is_value (fork e). *)
-  (* Axiom fork_inj : forall e1 e2, *)
-  (*                    fork e1 = fork e2 -> e1 = e2. *)
-
-  (** Evaluation contexts **)
-  (* Parameter ectx : Type. *)
-  (* Parameter empty_ctx : ectx. *)
-  (* Parameter comp_ctx : ectx -> ectx -> ectx. *)
-  (* Parameter fill : ectx -> expr -> expr. *)
-(*
-	All of
-		comp_ctx_assoc
-		comp_ctx_inj_r
-		comp_ctx_emp_r
-	arise only in the proof of
-
-		step_same_ctx K K' e e' :
-			fill K e = fill K' e' ->
-			reducible e  ->
-			reducible e' ->
-			K = K'.
-
-	Moreover, comp_ctx_positive gets used only in step_same_ctx
-	and
-
-		atomic_fill e K :
-			atomic (fill K e) ->
-			~ is_value e ->
-			K = empty_ctx.
-	
-	It might be simpler to (prove and) assume these two rather
-	than those four.
-*)
-  (* Axiom comp_ctx_emp_r : forall K, *)
-  (*   comp_ctx K empty_ctx = K. *)
-  (* Axiom comp_ctx_assoc : forall K0 K1 K2, *)
-  (*   comp_ctx K0 (comp_ctx K1 K2) = comp_ctx (comp_ctx K0 K1) K2. *)
-  (* Axiom comp_ctx_inj_r : forall K K1 K2, *)
-  (*   comp_ctx K K1 = comp_ctx K K2 -> K1 = K2. *)
-  (* Axiom comp_ctx_positive : forall K1 K2, *)
-  (*   comp_ctx K1 K2 = empty_ctx -> K1 = empty_ctx /\ K2 = empty_ctx. *)
-
-  (* Axiom fill_empty : forall e, fill empty_ctx e = e. *)
-  (* Axiom fill_comp  : forall K1 K2 e, fill K1 (fill K2 e) = fill (comp_ctx K1 K2) e. *)
-  (* Axiom fill_inj_r  : forall K e1 e2, fill K e1 = fill K e2 -> e1 = e2. *)
-  (* Axiom fill_value : forall K e, is_value (fill K e) -> is_value e. *)
-  (* Axiom fill_fork : forall K e e', fork e' = fill K e -> K = empty_ctx. *)
-
   (** Shared machine state (e.g., the heap) **)
   Parameter state : Type.
 
   (** Primitive (single thread) machine configurations **)
   Definition prim_cfg : Type := (expr * state)%type.
-
-  Definition thread_id := nat.
   
-  (** The primitive atomic stepping relation **)
+  (** The primitive atomic optionally-forking stepping relation **)
   Parameter prim_step : prim_cfg -> prim_cfg -> option expr -> Prop.
 
+  (** Some derived notions **)
   Definition reducible e: Prop :=
-    exists sigma cfg' oe, prim_step (e, sigma) cfg' oe.
+    exists sigma cfg' ef, prim_step (e, sigma) cfg' ef.
 
   Definition stuck (e : expr) : Prop :=
       ~reducible e.
 
-  (* Axiom fork_stuck : *)
-  (*   forall K e, stuck (fill K (fork e) ). *)
-  Axiom values_stuck :
-    forall e, is_value e -> stuck e.
-
-  (* When something does a step, and another decomposition of the same
-     expression has a non-value e in the hole, then K is a left
-     sub-context of K' - in other words, e also contains the reducible
-     expression *)
-  (* Axiom step_by_value : *)
-  (*   forall K K' e e', *)
-  (*     fill K e = fill K' e' -> *)
-  (*     reducible e' -> *)
-  (*     ~ is_value e -> *)
-  (*     exists K'', K' = comp_ctx K K''. *)
-  (* (* Similar to above, buth with a fork instead of a reducible *)
-  (*    expression *) *)
-  (* Axiom fork_by_value : *)
-  (*   forall K K' e e', *)
-  (*     fill K e = fill K' (fork e') -> *)
-  (*     ~ is_value e -> *)
-  (*     exists K'', K' = comp_ctx K K''. *)
-
   (** Atomic expressions **)
   Parameter atomic : expr -> Prop.
 
-  Axiom atomic_reducible :
-    forall e, atomic e -> reducible e.
+  (** Things ought to make sense. **)
+  Axiom values_stuck :
+    forall e, is_value e -> stuck e.
 
-  Axiom atomic_step: forall e σ e' σ' oe,
+  Axiom atomic_not_value :
+    forall e, atomic e -> ~is_value e.
+
+  Axiom atomic_step: forall e σ e' σ' ef,
                        atomic e ->
-                       prim_step (e, σ) (e', σ') oe ->
+                       prim_step (e, σ) (e', σ') ef ->
                        is_value e'.
 
 End CORE_LANG.
